Diamond.dfy
@@ -1,0 +1,407 @@
+include "Confluence.dfy"
+include "BetaReduction.dfy"
+
+lemma {:vcs_split_on_every_assert}DiamondLemma (M:LambdaTerm,M1:LambdaTerm,M2:LambdaTerm)
+    requires parallelReduction(M,M1)
+    requires parallelReduction(M,M2)
+    ensures exists M3:LambdaTerm::parallelReduction(M1,M3) && parallelReduction(M2,M3)
+    decreases lHeight(M)
+{
+
+    assert (alphaEquivalence(M,M1) || rule2(M,M1) || rule3(M,M1) || rule4(M,M1)) <==> parallelReduction(M,M1);
+    if (alphaEquivalence(M,M1))
+    {
+        EqualTermsAreAlphaEquilvalent(M2,M2);
+        ParallelReductionAlphaInvariance(M,M2,M1,M2);
+        var M3:=M2;
+        assert parallelReduction(M1,M3) && parallelReduction(M2,M3);
+    }
+    else 
+    {
+        if (rule3(M,M1))
+        {
+            match M 
+                case Application(P,Q) =>
+                {
+                    match M1
+                        case Application(P',Q') =>
+                        {
+                            assert parallelReduction(P,P');
+                            assert parallelReduction(Q,Q');
+
+                            assert parallelReduction(Application(P,Q),M2);
+
+                            AlphaParallelLemma(P,Q,M2);
+                            var part1:=(exists P'2: LambdaTerm, Q'2: LambdaTerm :: 
+                            parallelReduction(P, P'2) && parallelReduction(Q, Q'2) && alphaEquivalence(Application(P'2, Q'2), M2));
+                            if (part1)
+                            {
+                                var P'2:LambdaTerm,Q'2:LambdaTerm :|parallelReduction(P, P'2) && 
+                                parallelReduction(Q, Q'2) && alphaEquivalence(Application(P'2, Q'2), M2);
+
+                                assert parallelReduction(P,P');
+                                assert parallelReduction(P,P'2);
+                                DiamondLemma(P,P',P'2);
+                                var P'3:| parallelReduction(P',P'3) && parallelReduction(P'2,P'3);
+
+                                assert parallelReduction(Q,Q');
+                                assert parallelReduction(Q,Q'2);
+                                DiamondLemma(Q,Q',Q'2);
+                                var Q'3:| parallelReduction(Q',Q'3) && parallelReduction(Q'2,Q'3);
+
+                                var right_result:=Application(P'2,Q'2);
+                                var M3:=Application(P'3,Q'3);
+
+                                assert parallelReduction(Q'2,Q'3) && parallelReduction(P'2,P'3);
+                                assert rule3(right_result,M3);
+                                EqualTermsAreAlphaEquilvalent(M3,M3);
+                                ParallelReductionAlphaInvariance(right_result,M3,M2,M3);
+
+                                assert parallelReduction(M2,M3); 
+
+                                assert parallelReduction(Q',Q'3) && parallelReduction(P',P'3);
+
+                                assert rule3(M1,M3);
+
+                                assert parallelReduction(M1,M3) && parallelReduction(M2,M3);
+                            }
+                            else 
+                            {
+                                assert (P.Lambda? && 
+                                        exists P1'': LambdaTerm, Q'': LambdaTerm :: 
+                                            parallelReduction(P.t, P1'') 
+                                            && parallelReduction(Q, Q'') 
+                                            && alphaEquivalence(M2, caSubstitution(P1'', P.x, Q'')));
+
+                                var P1:LambdaTerm,x:Id:|P==Lambda(x,P1);
+
+                                var P1'2:LambdaTerm,Q'2:LambdaTerm :| parallelReduction(P.t, P1'2) 
+                                            && parallelReduction(Q, Q'2) 
+                                            && alphaEquivalence(M2, caSubstitution(P1'2, P.x, Q'2));
+
+
+                                assert parallelReduction(P,P'); 
+                                LambdaParallelLemma(P1,P',x);
+                                
+                                var P1':LambdaTerm:| parallelReduction(P1,P1') && alphaEquivalence(Lambda(x,P1'),P');
+                                var P'_result:=Lambda(x,P1');
+
+                                assert parallelReduction(P1,P1') && parallelReduction(P1,P1'2);
+                                assert parallelReduction(Q,Q') && parallelReduction(Q,Q'2);
+
+                                assert lHeight(P1)<lHeight(Lambda(x,P1))==lHeight(P)<lHeight(M);
+                                DiamondLemma(P1,P1',P1'2);
+                                DiamondLemma(Q,Q',Q'2);
+
+                                var P1'3:LambdaTerm:|parallelReduction(P1',P1'3) && parallelReduction(P1'2,P1'3);
+                                var Q'3:LambdaTerm:|parallelReduction(Q',Q'3) && parallelReduction(Q'2,Q'3);
+
+                                EqualTermsAreAlphaEquilvalent(Q',Q');
+                                AlphaEquivSymmetric(P'_result,P');
+                                ApplicationEquivalence(P',P'_result,Q',Q');
+                                var M1_result:=Application(P'_result,Q');
+                                assert alphaEquivalence(M1,M1_result);
+
+                                var M3 := caSubstitution(P1'3, x, Q'3);
+                                assert alphaEquivalence(M2, caSubstitution(P1'2, x, Q'2));
+
+
+                                EqualTermsAreAlphaEquilvalent(M3,M3);
+                                assert rule4(M1_result, M3) by {
+                                    assert parallelReduction(P1', P1'3);
+                                    assert parallelReduction(Q', Q'3);
+                                    assert alphaEquivalence(M3, caSubstitution(P1'3, x, Q'3));
+                                }
+
+                                assert parallelReduction(M1_result,M3);
+
+                                AlphaEquivSymmetric(M1, M1_result);
+                                ParallelReductionAlphaInvariance(M1_result, M3, M1, M3);
+
+                                ParallelReductionMultiSubstitution(P1'2, Q'2, P1'3, Q'3, x);
+                                AlphaEquivSymmetric(M2, caSubstitution(P1'2, x, Q'2));
+                                ParallelReductionAlphaInvariance(caSubstitution(P1'2, x, Q'2), M3, M2, M3);
+
+                                assert parallelReduction(M1, M3) && parallelReduction(M2, M3);
+                            }
+                        }
+                }
+                case _ => 
+                {
+                    assert false;
+                }
+        }
+        else 
+        {
+            if (rule4(M,M1))
+            {
+                assert M.Application?;
+                assert M.t1.Lambda?;
+
+                var x:Id,P:LambdaTerm,Q:LambdaTerm :| M==Application(Lambda(x,P),Q);
+
+                var P':LambdaTerm,Q':LambdaTerm:| parallelReduction(P,P') && parallelReduction(Q,Q') && alphaEquivalence(M1,caSubstitution(P',x,Q'));
+
+                AlphaParallelLemma(Lambda(x,P),Q,M2);
+
+                var part1:=        (exists P'2_temp: LambdaTerm, Q'2: LambdaTerm :: 
+                parallelReduction(Lambda(x,P),P'2_temp) && parallelReduction(Q, Q'2) && alphaEquivalence(Application(P'2_temp, Q'2), M2));
+
+                if (part1)
+                {
+                    var P'2_temp: LambdaTerm, Q'2: LambdaTerm :|
+                        parallelReduction(Lambda(x,P),P'2_temp) && parallelReduction(Q, Q'2) && alphaEquivalence(Application(P'2_temp, Q'2), M2);
+
+                    LambdaParallelLemma(P,P'2_temp,x);
+                    var P'2: LambdaTerm :| parallelReduction(P, P'2) && alphaEquivalence(Lambda(x, P'2), P'2_temp);
+
+                    assert parallelReduction(P,P'2) && parallelReduction(P,P');
+                    assert parallelReduction(Q,Q'2) && parallelReduction(Q,Q');
+
+                    assert lHeight(P)<lHeight(Lambda(x,P))<lHeight(M);
+                    DiamondLemma(P,P',P'2);
+                    DiamondLemma(Q,Q',Q'2);
+
+                    var P'3:|parallelReduction(P',P'3) && parallelReduction(P'2,P'3);
+                    var Q'3:|parallelReduction(Q',Q'3) && parallelReduction(Q'2,Q'3); 
+
+                    var M1_new:=caSubstitution(P',x,Q');
+                    var M3:=caSubstitution(P'3,x,Q'3);
+                    ParallelReductionMultiSubstitution(P',Q',P'3,Q'3,x);
+                    ParallelReductionMultiSubstitution(P'2,Q'2,P'3,Q'3,x);
+
+                    assert parallelReduction(M1_new,M3);
+                    EqualTermsAreAlphaEquilvalent(M3,M3);
+
+                    AlphaEquivSymmetric(M1,M1_new);
+                    ParallelReductionAlphaInvariance(M1_new,M3,M1,M3);
+
+                    assert parallelReduction(M1,M3);
+
+                    assert rule4(Application(Lambda(x,P'2),Q'2),M3)==true;
+
+                    EqualTermsAreAlphaEquilvalent(Q'2,Q'2);
+
+                    assert alphaEquivalence(Lambda(x, P'2), P'2_temp); 
+                    assert alphaEquivalence(Q'2,Q'2);
+
+                    ApplicationEquivalence(Lambda(x,P'2),P'2_temp,Q'2,Q'2) by {
+                        assert alphaEquivalence(Lambda(x, P'2), P'2_temp); 
+                        assert alphaEquivalence(Q'2,Q'2);
+                }
+
+                    
+                    var M2_result_2:=Application(Lambda(x, P'2),Q'2);
+
+                    var M2_result_1:=Application(P'2_temp,Q'2);
+
+                    assert alphaEquivalence(M2_result_2,M2_result_1);
+
+                    assert alphaEquivalence(Application(P'2_temp, Q'2), M2);
+                    assert alphaEquivalence(M2_result_1,M2);
+
+                    AlphaEquivTransitive(M2_result_2,M2_result_1,M2);
+
+                    ParallelReductionAlphaInvariance(M2_result_2,M3,M2,M3);
+
+                    assert parallelReduction(M2,M3) ;
+                    assert parallelReduction(M1,M3);
+
+                }
+                else 
+                {
+                    assert  (Lambda(x,P).Lambda? && 
+                        exists P'2: LambdaTerm, Q'2: LambdaTerm :: 
+                             parallelReduction(P, P'2) && parallelReduction(Q, Q'2) && alphaEquivalence(M2, caSubstitution(P'2, x, Q'2)));
+
+                    assert exists P'2: LambdaTerm, Q'2: LambdaTerm :: 
+                             parallelReduction(P, P'2) && parallelReduction(Q, Q'2) && alphaEquivalence(M2, caSubstitution(P'2, x, Q'2));
+
+                    var P'2: LambdaTerm, Q'2: LambdaTerm :| 
+                             parallelReduction(P, P'2) && parallelReduction(Q, Q'2) && alphaEquivalence(M2, caSubstitution(P'2, x, Q'2));
+
+                    assert parallelReduction(P,P') && parallelReduction(P,P'2);
+                    assert parallelReduction(Q,Q') && parallelReduction(Q,Q'2);
+
+                    assert lHeight(P)<lHeight(Lambda(x,P))<lHeight(M);
+                    DiamondLemma(P,P',P'2);
+                    DiamondLemma(Q,Q',Q'2);
+
+                    var P'3:LambdaTerm:|parallelReduction(P',P'3) && parallelReduction(P'2,P'3);
+                    var Q'3:LambdaTerm:|parallelReduction(Q',Q'3) && parallelReduction(Q'2,Q'3);
+
+                    var M1_new:=caSubstitution(P',x,Q');
+
+                    assert alphaEquivalence(M1,M1_new);
+                    AlphaEquivSymmetric(M1,M1_new);
+
+                    assert parallelReduction(P',P'3);
+                    assert parallelReduction(Q',Q'3);
+
+                    ParallelReductionMultiSubstitution(P',Q',P'3,Q'3,x) ;
+
+                    var M3:=caSubstitution(P'3,x,Q'3);
+
+                    assert parallelReduction(M1_new,M3);
+
+                    EqualTermsAreAlphaEquilvalent(M3,M3);
+
+                    ParallelReductionAlphaInvariance(M1_new,M3,M1,M3);
+
+                    assert parallelReduction(M1,M3);    
+
+                    assert parallelReduction(P'2,P'3);
+                    assert parallelReduction(Q'2,Q'3);
+
+                    ParallelReductionMultiSubstitution(P'2,Q'2,P'3,Q'3,x) ;
+
+                    var M2_new:=caSubstitution(P'2,x,Q'2);
+                    assert  alphaEquivalence(M2, M2_new);
+                    AlphaEquivSymmetric(M2,M2_new);
+
+                    assert parallelReduction(M2_new,M3);
+                    ParallelReductionAlphaInvariance(M2_new,M3,M2,M3);
+
+                    assert parallelReduction(M2,M3);
+                }
+
+            }  
+            else 
+            {
+                assert rule2(M,M1);
+                match M 
+                    case Lambda(x,P) =>
+                    {
+                        assert    exists P': LambdaTerm ::
+                                parallelReduction(P, P') && alphaEquivalence(Lambda(x, P'), M1);
+                        var P': LambdaTerm :|
+                                parallelReduction(P, P') && alphaEquivalence(Lambda(x, P'), M1);
+                        
+                        var M1_new:=Lambda(x,P');
+
+                        LambdaParallelLemma(P,M2,x);
+                        assert exists P'2: LambdaTerm :: parallelReduction(P, P'2) && alphaEquivalence(Lambda(x, P'2), M2) ;
+                            
+                        var P'2:LambdaTerm:| parallelReduction(P, P'2) && alphaEquivalence(Lambda(x, P'2), M2);
+
+                        var M2_new:=Lambda(x, P'2);
+                        assert alphaEquivalence(M2_new,M2);
+
+                        assert parallelReduction(P,P');
+                        assert parallelReduction(P,P'2);
+
+                        assert lHeight(P)<lHeight(M);
+                        DiamondLemma(P,P',P'2);
+
+                        var P'3:|parallelReduction(P',P'3) && parallelReduction(P'2,P'3);
+
+                        var M3:=Lambda(x,P'3);
+                        
+                        EqualTermsAreAlphaEquilvalent(M3,M3);
+                        assert rule2(M1_new,M3);
+                        assert rule2(M2_new,M3);
+
+                        assert parallelReduction(M1_new,M3);
+                        assert parallelReduction(M2_new,M3);
+                        ParallelReductionAlphaInvariance(M1_new,M3,M1,M3);
+                        ParallelReductionAlphaInvariance(M2_new,M3,M2,M3);
+                        assert parallelReduction(M1,M3) && parallelReduction(M2,M3);
+
+                    }
+            }
+        }
+    }
+}
+
+ghost predicate parallelReductionInNSteps(t1:LambdaTerm,t2:LambdaTerm,n:nat)
+    decreases n
+{
+    if n==0 then alphaEquivalence(t1,t2)
+    else 
+    exists t':LambdaTerm:: parallelReduction(t1,t') && parallelReductionInNSteps(t',t2,n-1)
+}
+
+ghost predicate parallelReductionClosure(t1:LambdaTerm,t2:LambdaTerm)
+{
+    exists n:nat::parallelReductionInNSteps(t1,t2,n)
+}
+
+lemma parallelReductionClosureReflexive(t1:LambdaTerm)
+    ensures parallelReductionClosure(t1,t1)
+{
+    EqualTermsAreAlphaEquilvalent(t1,t1);
+    assert alphaEquivalence(t1,t1);
+    assert parallelReductionInNSteps(t1,t1,0);
+}
+lemma ParClosurePrepend(a:LambdaTerm, b:LambdaTerm, c:LambdaTerm)   
+    requires parallelReduction(a, b)
+    requires parallelReductionClosure(b, c)
+    ensures parallelReductionClosure(a, c)
+{
+    var n:nat :| parallelReductionInNSteps(b, c, n);
+    assert parallelReductionInNSteps(a, c, n+1);     
+}
+lemma StripLemma(a:LambdaTerm,b:LambdaTerm,c:LambdaTerm,n:nat)
+    requires parallelReduction(a, b)
+    requires parallelReductionInNSteps(a, c, n)
+    ensures exists d:LambdaTerm ::parallelReductionClosure(b, d) && parallelReduction(c, d)
+    decreases n
+{
+    if n==0{
+        assert alphaEquivalence(a,c);
+        assert parallelReduction(a,b);
+        EqualTermsAreAlphaEquilvalent(b,b);
+        ParallelReductionAlphaInvariance(a,b,c,b);
+        assert parallelReduction(b,b);
+        assert parallelReduction(c,b);
+        assert parallelReductionInNSteps(b,b,0);
+        assert parallelReductionInNSteps(c,b,1);
+
+    }
+    else
+    {
+        var a1 :| parallelReduction(a, a1) && parallelReductionInNSteps(a1, c, n-1);
+        DiamondLemma(a, b, a1);                    
+        var e :| parallelReduction(b, e) && parallelReduction(a1, e);
+        StripLemma(a1, e, c, n-1);                  
+        var d :| parallelReductionClosure(e, d) && parallelReduction(c, d);
+        ParClosurePrepend(b, e, d);                    
+        assert parallelReductionClosure(b, d) && parallelReduction(c, d);
+    }
+}
+
+lemma ClosureDiamond(a:LambdaTerm, b:LambdaTerm, c:LambdaTerm, m:nat)
+    requires parallelReductionInNSteps(a, b, m)
+    requires parallelReductionClosure(a, c)
+    ensures exists d:LambdaTerm :: parallelReductionClosure(b, d) && parallelReductionClosure(c, d)
+    decreases m 
+{
+    if (m==0)
+    {
+        assert alphaEquivalence(a, b);
+        AlphaEquivSymmetric(a, b);                
+        ParClosurePrepend(b, a, c);                
+        parallelReductionClosureReflexive(c);     
+        assert parallelReductionClosure(b, c) && parallelReductionClosure(c, c);
+        
+    }
+    else
+    {
+        var a1 :| parallelReduction(a, a1) && parallelReductionInNSteps(a1, b, m-1);
+        var k:nat :| parallelReductionInNSteps(a, c, k);
+        StripLemma(a, a1, c, k);                    
+        var e :| parallelReductionClosure(a1, e) && parallelReduction(c, e);
+        ClosureDiamond(a1, b, e, m-1);             
+        var d :| parallelReductionClosure(b, d) && parallelReductionClosure(e, d);
+        ParClosurePrepend(c, e, d);                
+        assert parallelReductionClosure(b, d) && parallelReductionClosure(c, d);
+    }
+}
+lemma ParallelClosureHasDiamond(a:LambdaTerm, b:LambdaTerm, c:LambdaTerm)
+    requires parallelReductionClosure(a, b)
+    requires parallelReductionClosure(a, c)
+    ensures exists d:LambdaTerm :: parallelReductionClosure(b, d) && parallelReductionClosure(c, d)
+{
+    var m:nat :| parallelReductionInNSteps(a, b, m);
+    ClosureDiamond(a, b, c, m);
+}
