TuringMachine/example.dfy
@@ -1,0 +1,173 @@
+include "DTM.dfy"
+
+function getInputOfN (n:nat):seq<string>
+  requires n>=0
+  decreases n
+{
+  if n==0 then 
+    []
+  else
+    ["1"]+getInputOfN(n-1)
+}
+predicate isInputCorrect (input:seq<string>)
+  ensures isInputCorrect(input) ==> forall n:nat:: n<|input| ==> input[n]=="1"
+  decreases input 
+{
+ if input==[] then true
+ else 
+    input[0]=="1" && isInputCorrect(input[1..])
+}
+function finalStateForInput (input:seq<string>) :State
+{
+  if |input|%2==0 then 
+    State("qAcc", Some(Accept))
+  else 
+    State("qRej", Some(Reject))
+
+}
+function finalTapeForExample() : iseq<Symbol>
+{
+    i =>
+        Blank
+}
+lemma TraceExecution(
+  delta: DeterministicTransitions,
+  inputS: InputSymbols,
+  addTapeS: AdditionalTapeSymbols,
+  current_conf: Configuration,
+  n: nat
+) returns (next_conf: Configuration)
+  requires isTapeSymbolsValid(inputS, addTapeS)
+  requires isDeterministicTransitionsValid(delta, inputS, addTapeS)
+  requires {Key(State("q0", None), NonBlankSymbol("1")), Key(State("q1", None), NonBlankSymbol("1"))} <= delta.Keys
+  requires delta[Key(State("q0", None), NonBlankSymbol("1"))] == Action(State("q1", None), Blank, Right)
+  requires delta[Key(State("q1", None), NonBlankSymbol("1"))] == Action(State("q0", None), Blank, Right)
+  requires current_conf.s == State("q0", None) || current_conf.s == State("q1", None)
+  requires forall i :: current_conf.head <= i < current_conf.head + n ==> current_conf.tape(i) == NonBlankSymbol("1")
+  requires current_conf.tape(current_conf.head + n) == Blank
+  decreases n
+  ensures next_conf.head == current_conf.head + n
+  ensures next_conf.tape(next_conf.head) == Blank
+  ensures next_conf.s == State("q0", None) || next_conf.s == State("q1", None)
+  ensures isThereAClosedTransitionInNStepsForDTM(delta, inputS, addTapeS, current_conf, next_conf, n)
+{
+  if n == 0 {
+    next_conf := current_conf;
+  } else {
+    match applyTransitionDTM(current_conf, delta)
+      case Some(step_conf) => {
+        next_conf := TraceExecution(delta, inputS, addTapeS, step_conf, n - 1);
+      }
+      case None => { }
+  }
+}
+
+lemma CorrectInputHalts(
+  delta: DeterministicTransitions, 
+  inputS: InputSymbols, 
+  addTapeS: AdditionalTapeSymbols, 
+  q0: State, 
+  q1: State, 
+  qRej: State, 
+  qAcc: State,
+  one: Symbol, 
+  input: seq<string>
+)
+  requires isInputCorrect(input)
+  requires |input| >= 1
+  requires one == NonBlankSymbol("1")
+  requires inputS == {one}
+  requires addTapeS == {Blank}
+  requires isTapeSymbolsValid(inputS, addTapeS)
+  requires isInputValid(input, inputS)
+  requires isDeterministicTransitionsValid(delta, inputS, addTapeS)
+  requires q0 == State("q0", None)
+  requires q1 == State("q1", None)
+  requires qRej == State("qRej", Some(Reject))
+  requires qAcc == State("qAcc", Some(Accept))
+  requires {Key(q0, one), Key(q1, one), Key(q1, Blank), Key(q0, Blank)} <= delta.Keys
+  requires delta[Key(q0, one)] == Action(q1, Blank, Right)
+  requires delta[Key(q1, one)] == Action(q0, Blank, Right)
+  requires delta[Key(q1, Blank)] == Action(qRej, Blank, Right)
+  requires delta[Key(q0, Blank)] == Action(qAcc, Blank, Right)
+  ensures haltsInDTM(delta, q0, inputS, addTapeS, input)
+{
+  var init_config := initialConfiguration(input, q0, inputS);
+  var steps := |input|;
+
+  var mid_config := TraceExecution(delta, inputS, addTapeS, init_config, steps);
+  
+  match applyTransitionDTM(mid_config, delta)
+    case Some(halt_config) => {
+      LinkTransitions(delta, inputS, addTapeS, init_config, mid_config, halt_config, steps);
+
+      assert isThereAClosedTransitionInNStepsForDTM(delta, inputS, addTapeS, init_config, halt_config, steps + 1);
+      assert isThereAClosedTransitionDTM(delta,inputS,addTapeS,init_config,halt_config);
+      assert haltsInDTM(delta, q0, inputS, addTapeS, input);
+    }
+    case None => {}
+}
+
+lemma LinkTransitions(
+  delta: DeterministicTransitions, 
+  inputS: InputSymbols, 
+  addTapeS: AdditionalTapeSymbols, 
+  c1: Configuration, 
+  c2: Configuration, 
+  c3: Configuration, 
+  n: nat
+)
+  requires isTapeSymbolsValid(inputS, addTapeS)
+  requires isDeterministicTransitionsValid(delta, inputS, addTapeS)
+  requires isThereAClosedTransitionInNStepsForDTM(delta, inputS, addTapeS, c1, c2, n)
+  requires applyTransitionDTM(c2, delta) == Some(c3)
+  ensures isThereAClosedTransitionInNStepsForDTM(delta, inputS, addTapeS, c1, c3, n + 1)
+  decreases n
+{
+  if n == 0 {
+  } else {
+    var c_prime :| applyTransitionDTM(c1, delta) == Some(c_prime) && 
+                   isThereAClosedTransitionInNStepsForDTM(delta, inputS, addTapeS, c_prime, c2, n-1);
+    LinkTransitions(delta, inputS, addTapeS, c_prime, c2, c3, n - 1);
+  }
+}
+method Main()
+{
+  var q0:=State("q0",None);
+  var q1:=State("q1",None);
+  var qAcc:=State("qAcc",Some(Accept));
+  var qRej:=State("qRej",Some(Reject));
+  var one:=NonBlankSymbol("1");
+  var delta:= map[
+    Key(q0,one) :=[Action(q1,Blank,Right)],
+    Key(q1,one) := [Action(q0,Blank,Right)],
+    Key(q0,Blank) := [Action(qAcc,Blank,Right)],
+    Key(q1,Blank) := [Action(qRej,Blank,Right)]
+  ];
+  assert one==NonBlankSymbol("1");
+  var input:=["1","1","1","1","1"];
+  var inputS:={one};
+  var addTapeS:={Blank};
+  print input;
+  print "\n";
+
+
+  assert isTapeSymbolsValid(inputS, addTapeS);
+  assert isInputValid(input, inputS);
+  assert isTransitionsValid(delta, inputS, addTapeS);
+  assert isTransitionsDeterministic(delta, inputS, addTapeS);
+  
+  var deltaDTM := fromNDTMtoDTM(delta, inputS, addTapeS);
+
+  
+
+
+  CorrectInputHalts(deltaDTM, inputS, addTapeS, q0, q1, qRej,qAcc,one,input);
+
+
+
+  assert haltsInDTM(deltaDTM, q0, inputS, addTapeS, input);
+
+  var finalConfig := beginDTM(deltaDTM, inputS, addTapeS, q0, input);
+
+}
